# baseURI: http://lpis.csd.auth.gr/ontologies/2015/CSSP.ttl
# imports: http://lpis.csd.auth.gr/ontologies/2015/DSO.ttl
# imports: http://lpis.csd.auth.gr/ontologies/2015/PRP
# imports: http://lpis.csd.auth.gr/ontologies/2015/RBLP
# imports: http://spinrdf.org/spin

@prefix CSSP: <http://lpis.csd.auth.gr/ontologies/2015/CSSP.ttl#> .
@prefix owl: <http://www.w3.org/2002/07/owl#> .
@prefix rdf: <http://www.w3.org/1999/02/22-rdf-syntax-ns#> .
@prefix rdfs: <http://www.w3.org/2000/01/rdf-schema#> .
@prefix sp: <http://spinrdf.org/sp#> .
@prefix spin: <http://spinrdf.org/spin#> .
@prefix xsd: <http://www.w3.org/2001/XMLSchema#> .

<http://lpis.csd.auth.gr/ontologies/2015/CSSP.ttl>
  rdf:type owl:Ontology ;
  spin:imports <http://topbraid.org/spin/rdfsplus> ;
  owl:imports <http://lpis.csd.auth.gr/ontologies/2015/DSO.ttl> ;
  owl:imports <http://lpis.csd.auth.gr/ontologies/2015/PRP> ;
  owl:imports <http://lpis.csd.auth.gr/ontologies/2015/RBLP> ;
  owl:imports <http://spinrdf.org/spin> ;
  owl:versionInfo "Created with TopBraid Composer"^^xsd:string ;
.
CSSP:AbstractRequirement
  rdf:type owl:Class ;
  spin:rule [
      rdf:type sp:Construct ;
      sp:templates (
          [
            sp:object [
                sp:varName "e"^^xsd:string ;
              ] ;
            sp:predicate CSSP:hasAbstractEntity ;
            sp:subject spin:_this ;
          ]
        ) ;
      sp:where (
          [
            sp:object [
                sp:varName "x"^^xsd:string ;
              ] ;
            sp:predicate CSSP:hasClause ;
            sp:subject spin:_this ;
          ]
          [
            rdf:type sp:TriplePath ;
            sp:object [
                sp:varName "e"^^xsd:string ;
              ] ;
            sp:path [
                rdf:type sp:ModPath ;
                sp:modMax -2 ;
                sp:modMin 1 ;
                sp:subPath <http://lpis.csd.auth.gr/ontologies/2015/RBLP#isRelatedToAttribute> ;
              ] ;
            sp:subject [
                sp:varName "x"^^xsd:string ;
              ] ;
          ]
          [
            sp:object owl:Class ;
            sp:predicate rdf:type ;
            sp:subject [
                sp:varName "e"^^xsd:string ;
              ] ;
          ]
        ) ;
    ] ;
  spin:rule [
      rdf:type sp:Construct ;
      sp:templates (
          [
            sp:object [
                sp:varName "e"^^xsd:string ;
              ] ;
            sp:predicate CSSP:mainAbstractEntity ;
            sp:subject spin:_this ;
          ]
        ) ;
      sp:where (
          [
            sp:object [
                sp:varName "x"^^xsd:string ;
              ] ;
            sp:predicate CSSP:hasMain ;
            sp:subject spin:_this ;
          ]
          [
            sp:object [
                sp:varName "e"^^xsd:string ;
              ] ;
            sp:predicate <http://lpis.csd.auth.gr/ontologies/2015/RBLP#isRelatedToSubject> ;
            sp:subject [
                sp:varName "x"^^xsd:string ;
              ] ;
          ]
          [
            sp:object owl:Class ;
            sp:predicate rdf:type ;
            sp:subject [
                sp:varName "e"^^xsd:string ;
              ] ;
          ]
        ) ;
    ] ;
  spin:rule [
      rdf:type sp:Construct ;
      sp:templates (
          [
            sp:object [
                sp:varName "e1"^^xsd:string ;
              ] ;
            sp:predicate CSSP:mainAbstractEntity ;
            sp:subject spin:_this ;
          ]
        ) ;
      sp:where (
          [
            sp:object [
                sp:varName "x"^^xsd:string ;
              ] ;
            sp:predicate CSSP:hasMain ;
            sp:subject spin:_this ;
          ]
          [
            sp:object [
                sp:varName "e"^^xsd:string ;
              ] ;
            sp:predicate <http://lpis.csd.auth.gr/ontologies/2015/RBLP#isRelatedToSubject> ;
            sp:subject [
                sp:varName "x"^^xsd:string ;
              ] ;
          ]
          [
            rdf:type sp:NotExists ;
            sp:elements (
                [
                  sp:object owl:Class ;
                  sp:predicate rdf:type ;
                  sp:subject [
                      sp:varName "e"^^xsd:string ;
                    ] ;
                ]
              ) ;
          ]
          [
            rdf:type sp:TriplePath ;
            sp:object [
                sp:varName "e1"^^xsd:string ;
              ] ;
            sp:path [
                rdf:type sp:ModPath ;
                sp:modMax -2 ;
                sp:modMin 1 ;
                sp:subPath <http://lpis.csd.auth.gr/ontologies/2015/RBLP#isRelatedToAttribute> ;
              ] ;
            sp:subject [
                sp:varName "x"^^xsd:string ;
              ] ;
          ]
          [
            sp:object owl:Class ;
            sp:predicate rdf:type ;
            sp:subject [
                sp:varName "e1"^^xsd:string ;
              ] ;
          ]
        ) ;
    ] ;
  rdfs:label "Abstract req"^^xsd:string ;
  rdfs:subClassOf CSSP:Requirement ;
.
CSSP:Acquisition-CommandingMinimumSeparationRequirement
  rdf:type owl:Class ;
  rdfs:comment "RB level:This category comprise requirements that impose a minimum separation between two acquisition or commanding activities."^^xsd:string ;
  rdfs:label "Acquisition-Commanding minimum separation requirement"^^xsd:string ;
  rdfs:subClassOf CSSP:PerformanceRequirements ;
  rdfs:subClassOf [
      rdf:type owl:Restriction ;
      owl:allValuesFrom <http://lpis.csd.auth.gr/ontologies/2015/OoSSA.ttl#RB> ;
      owl:onProperty CSSP:hasAbstractionLevel ;
    ] ;
.
CSSP:AcquisitionPriorityRequirement
  rdf:type owl:Class ;
  rdfs:comment "RB level: This category comprises requirements that imposes a priority on a given acquisition."^^xsd:string ;
  rdfs:label "Acquisition priority requirement"^^xsd:string ;
  rdfs:subClassOf CSSP:PerformanceRequirements ;
  rdfs:subClassOf [
      rdf:type owl:Restriction ;
      owl:allValuesFrom <http://lpis.csd.auth.gr/ontologies/2015/OoSSA.ttl#RB> ;
      owl:onProperty CSSP:hasAbstractionLevel ;
    ] ;
.
CSSP:AcquisitionRelativeOffsetRequirement
  rdf:type owl:Class ;
  rdfs:comment "RB level: This category comprise requirements that impose a relative offset w.r.t. an event or a time occurrence for executing a given activity."^^xsd:string ;
  rdfs:label "Acquisition relative offset requirement"^^xsd:string ;
  rdfs:subClassOf CSSP:PerformanceRequirements ;
  rdfs:subClassOf [
      rdf:type owl:Restriction ;
      owl:allValuesFrom <http://lpis.csd.auth.gr/ontologies/2015/OoSSA.ttl#RB> ;
      owl:onProperty CSSP:hasAbstractionLevel ;
    ] ;
.
CSSP:AcquisitionTimingandPerformanceRequirement
  rdf:type owl:Class ;
  rdfs:label "Acquisition timingand performance requirement"^^xsd:string ;
  rdfs:subClassOf CSSP:PerformanceRequirements ;
  rdfs:subClassOf [
      rdf:type owl:Restriction ;
      owl:allValuesFrom <http://lpis.csd.auth.gr/ontologies/2015/OoSSA.ttl#RB> ;
      owl:onProperty CSSP:hasAbstractionLevel ;
    ] ;
.
CSSP:Algorithmic-ProtocolRequirement
  rdf:type owl:Class ;
  rdfs:comment "RB level: Algorithmic / Protocol Requirements are requirements describing a specific algorithmic procedure to be implemented by the function, or some specific protocol implementation (intended as a sequence of actions, possibly conditional) to be provided by the function."^^xsd:string ;
  rdfs:label "Algorithmic-Protocol requirement"^^xsd:string ;
  rdfs:subClassOf CSSP:FunctionalRequirement ;
  rdfs:subClassOf [
      rdf:type owl:Restriction ;
      owl:allValuesFrom <http://lpis.csd.auth.gr/ontologies/2015/OoSSA.ttl#RB> ;
      owl:onProperty CSSP:hasAbstractionLevel ;
    ] ;
.
CSSP:AvionicsTopologyRequirement
  rdf:type owl:Class ;
  rdfs:comment "Avionics level: Avionics Topology Requirements specifies the structure and organisation of the avionics, with connection between different avionics units."^^xsd:string ;
  rdfs:label "Avionics topology requirement"^^xsd:string ;
  rdfs:subClassOf CSSP:FunctionalRequirement ;
  rdfs:subClassOf [
      rdf:type owl:Restriction ;
      owl:allValuesFrom <http://lpis.csd.auth.gr/ontologies/2015/OoSSA.ttl#Avionics> ;
      owl:onProperty CSSP:hasAbstractionLevel ;
    ] ;
.
CSSP:BudgetRequirement
  rdf:type owl:Class ;
  rdfs:comment "System spacecraft level: Budget requirements specifies envelopes on various aspects of the OBSW, typically CPU load, OBSW memory occupation, functions memory occupation, communication."^^xsd:string ;
  rdfs:label "Budget requirement"^^xsd:string ;
  rdfs:subClassOf CSSP:OnBoardSoftwareRequirement ;
  rdfs:subClassOf [
      rdf:type owl:Restriction ;
      owl:allValuesFrom <http://lpis.csd.auth.gr/ontologies/2015/OoSSA.ttl#SystemSpacecraft> ;
      owl:onProperty CSSP:hasAbstractionLevel ;
    ] ;
.
CSSP:CommandabilityRequirement
  rdf:type owl:Class ;
  rdfs:comment "Avionics level: This class of requirements gather requirements on the commandability of the avionics. They comprise some generic requirements applicable to several subsystems."^^xsd:string ;
  rdfs:label "Commandability requirement"^^xsd:string ;
  rdfs:subClassOf CSSP:DesignAndConstructionRequirement ;
  rdfs:subClassOf [
      rdf:type owl:Restriction ;
      owl:allValuesFrom <http://lpis.csd.auth.gr/ontologies/2015/OoSSA.ttl#Avionics> ;
      owl:onProperty CSSP:hasAbstractionLevel ;
    ] ;
.
CSSP:CommandabilityRequirements
  rdf:type owl:Class ;
  rdfs:comment "RB level: Commandability Requirements specifies how a given function shall be commanded."^^xsd:string ;
  rdfs:label "Commandability requirements"^^xsd:string ;
  rdfs:subClassOf CSSP:InterfaceRequirement ;
  rdfs:subClassOf [
      rdf:type owl:Restriction ;
      owl:allValuesFrom <http://lpis.csd.auth.gr/ontologies/2015/OoSSA.ttl#RB> ;
      owl:onProperty CSSP:hasAbstractionLevel ;
    ] ;
.
CSSP:CommandingPrecedenceConstraintRequirement
  rdf:type owl:Class ;
  rdfs:comment "RB level: This category comprises requirements related to commanding, and describes an activity or event that shall complete / occur before the commanding activity."^^xsd:string ;
  rdfs:label "Commanding precedence constraint requirement"^^xsd:string ;
  rdfs:subClassOf CSSP:PerformanceRequirements ;
  rdfs:subClassOf [
      rdf:type owl:Restriction ;
      owl:allValuesFrom <http://lpis.csd.auth.gr/ontologies/2015/OoSSA.ttl#RB> ;
      owl:onProperty CSSP:hasAbstractionLevel ;
    ] ;
.
CSSP:CommandingRelativeTimeWindowRequirement
  rdf:type owl:Class ;
  rdfs:comment "RB level: This category comprises requirements related to commanding, with the specification of a given time window to execute the activity."^^xsd:string ;
  rdfs:label "Commanding relative time window requirement"^^xsd:string ;
  rdfs:subClassOf CSSP:PerformanceRequirements ;
  rdfs:subClassOf [
      rdf:type owl:Restriction ;
      owl:allValuesFrom <http://lpis.csd.auth.gr/ontologies/2015/OoSSA.ttl#RB> ;
      owl:onProperty CSSP:hasAbstractionLevel ;
    ] ;
.
CSSP:ConcreteRequirement
  rdf:type owl:Class ;
  rdfs:label "Concrete req"^^xsd:string ;
  rdfs:subClassOf CSSP:Requirement ;
.
CSSP:ConditionalFunctionalCapabilityRequirement
  rdf:type owl:Class ;
  rdfs:comment "RB level: Conditional Functional Capability Requirement express functionality to be provided by the system only when a specific condition holds."^^xsd:string ;
  rdfs:label "Conditional functional capability requirement"^^xsd:string ;
  rdfs:subClassOf CSSP:FunctionalRequirement ;
  rdfs:subClassOf [
      rdf:type owl:Restriction ;
      owl:allValuesFrom <http://lpis.csd.auth.gr/ontologies/2015/OoSSA.ttl#RB> ;
      owl:onProperty CSSP:hasAbstractionLevel ;
    ] ;
.
CSSP:ContextSavingRequirement
  rdf:type owl:Class ;
  rdfs:comment "RB level: Context Saving Requirements describes how the context of execution of a function shall be persisted."^^xsd:string ;
  rdfs:label "Context saving requirement"^^xsd:string ;
  rdfs:subClassOf CSSP:InterfaceRequirement ;
  rdfs:subClassOf [
      rdf:type owl:Restriction ;
      owl:allValuesFrom <http://lpis.csd.auth.gr/ontologies/2015/OoSSA.ttl#RB> ;
      owl:onProperty CSSP:hasAbstractionLevel ;
    ] ;
.
CSSP:Data-dependentFunctionalRequirement
  rdf:type owl:Class ;
  rdfs:comment "RB level: Data-dependent Functional Requirements express expectations on the system behaviour depending on the input that is received. They are put in a separate class of requirements as their formalisation or link with properties may require to be addressed differently."^^xsd:string ;
  rdfs:label "Data-dependent functional requirement"^^xsd:string ;
  rdfs:subClassOf CSSP:FunctionalRequirement ;
  rdfs:subClassOf [
      rdf:type owl:Restriction ;
      owl:allValuesFrom <http://lpis.csd.auth.gr/ontologies/2015/OoSSA.ttl#RB> ;
      owl:onProperty CSSP:hasAbstractionLevel ;
    ] ;
.
CSSP:DataRepresentationRequirement
  rdf:type owl:Class ;
  rdfs:comment """RB level: Data Representation Requirements are the mirror case of “Data Value Requirements”. In this case they specify the representation format that shall be used for a given element.
This is typically used for compatibility with expected format of expected communication with hardware elements or sensor / actuators."""^^xsd:string ;
  rdfs:label "Data representation requirement"^^xsd:string ;
  rdfs:subClassOf CSSP:DesignAndConstructionRequirement ;
  rdfs:subClassOf [
      rdf:type owl:Restriction ;
      owl:allValuesFrom <http://lpis.csd.auth.gr/ontologies/2015/OoSSA.ttl#RB> ;
      owl:onProperty CSSP:hasAbstractionLevel ;
    ] ;
.
CSSP:DataStorageRequirement
  rdf:type owl:Class ;
  rdfs:comment "Avionics level: Data Storage Requirements specify functionalities related to the storage of data."^^xsd:string ;
  rdfs:label "Data storage requirement"^^xsd:string ;
  rdfs:subClassOf CSSP:FunctionalRequirement ;
  rdfs:subClassOf [
      rdf:type owl:Restriction ;
      owl:allValuesFrom <http://lpis.csd.auth.gr/ontologies/2015/OoSSA.ttl#Avionics> ;
      owl:onProperty CSSP:hasAbstractionLevel ;
    ] ;
.
CSSP:DataTransmissionRelativeTimeWindowRequirement
  rdf:type owl:Class ;
  rdfs:comment "RB level: Requirements for relative Time Windows for data transmission are gathered in this category."^^xsd:string ;
  rdfs:label "Data transmission relative time window requirement"^^xsd:string ;
  rdfs:subClassOf CSSP:PerformanceRequirements ;
  rdfs:subClassOf [
      rdf:type owl:Restriction ;
      owl:allValuesFrom <http://lpis.csd.auth.gr/ontologies/2015/OoSSA.ttl#RB> ;
      owl:onProperty CSSP:hasAbstractionLevel ;
    ] ;
.
CSSP:DataTransmissionRequirement
  rdf:type owl:Class ;
  rdfs:comment "Avionics level: Data Transmission requirements gather all requirements related to transmission of data between avionics units."^^xsd:string ;
  rdfs:label "Data transmission requirement"^^xsd:string ;
  rdfs:subClassOf CSSP:PerformanceRequirements ;
  rdfs:subClassOf [
      rdf:type owl:Restriction ;
      owl:allValuesFrom <http://lpis.csd.auth.gr/ontologies/2015/OoSSA.ttl#Avionics> ;
      owl:onProperty CSSP:hasAbstractionLevel ;
    ] ;
.
CSSP:DataValueRequirement
  rdf:type owl:Class ;
  rdfs:comment "RB level: Data Value Requirements specify the expected range of values that shall be supported in the implementation for a given software element."^^xsd:string ;
  rdfs:label "Data value requirement"^^xsd:string ;
  rdfs:subClassOf CSSP:DesignAndConstructionRequirement ;
  rdfs:subClassOf [
      rdf:type owl:Restriction ;
      owl:allValuesFrom <http://lpis.csd.auth.gr/ontologies/2015/OoSSA.ttl#RB> ;
      owl:onProperty CSSP:hasAbstractionLevel ;
    ] ;
.
CSSP:DependabilityRequirement
  rdf:type owl:Class ;
  rdfs:comment "System spacecraft level: Dependability requirements regard dependability provisions or guarantees of the spacecraft as a whole, its functions, or of units."^^xsd:string ;
  rdfs:label "Dependability requirement"^^xsd:string ;
  rdfs:subClassOf CSSP:Requirement ;
  rdfs:subClassOf [
      rdf:type owl:Restriction ;
      owl:allValuesFrom <http://lpis.csd.auth.gr/ontologies/2015/OoSSA.ttl#SystemSpacecraft> ;
      owl:onProperty CSSP:hasAbstractionLevel ;
    ] ;
.
CSSP:DesignAndConstructionRequirement
  rdf:type owl:Class ;
  rdfs:comment """System spacecraft level: Design and construction requirements specifies specific conditions that shall be respected when designing, implementing or constructing the spacecraft.

Avionics level: Design and construction requirements imposes some specific constraints on the implementation of given subsystems or functions."""^^xsd:string ;
  rdfs:label "Design and construction requirement"^^xsd:string ;
  rdfs:subClassOf CSSP:Requirement ;
  rdfs:subClassOf [
      rdf:type owl:Restriction ;
      owl:allValuesFrom [
          rdf:type owl:Class ;
          owl:unionOf (
              <http://lpis.csd.auth.gr/ontologies/2015/OoSSA.ttl#SystemSpacecraft>
              <http://lpis.csd.auth.gr/ontologies/2015/OoSSA.ttl#Avionics>
              <http://lpis.csd.auth.gr/ontologies/2015/OoSSA.ttl#RB>
              <http://lpis.csd.auth.gr/ontologies/2015/OoSSA.ttl#TS>
            ) ;
        ] ;
      owl:onProperty CSSP:hasAbstractionLevel ;
    ] ;
.
CSSP:ExternalDefinitionRequirement
  rdf:type owl:Class ;
  rdfs:comment "RB level: These requirements require that the values of given configuration parameters are taken from an external input (typically the spacecraft database)."^^xsd:string ;
  rdfs:label "External definition requirement"^^xsd:string ;
  rdfs:subClassOf CSSP:DesignAndConstructionRequirement ;
  rdfs:subClassOf [
      rdf:type owl:Restriction ;
      owl:allValuesFrom <http://lpis.csd.auth.gr/ontologies/2015/OoSSA.ttl#RB> ;
      owl:onProperty CSSP:hasAbstractionLevel ;
    ] ;
.
CSSP:FDIRRequirement-DetectionandIdentification
  rdf:type owl:Class ;
  rdfs:comment """Avionics level: FDIR Requirements for Detection and Handling specifies what type of faults shall be detected and identified by subsystems of units or specifies the generic capabilities regarding Fault Detection and Identification that shall be implemented.

RB level: FDIR requirement related to detection of faults / errors / failures typically either enumerate the faults / errors / failures to be detected, or specifies how a fault shall be detected.
"""^^xsd:string ;
  rdfs:label "FDIRRequirement-Detectionand identification"^^xsd:string ;
  rdfs:subClassOf CSSP:FunctionalRequirement ;
  rdfs:subClassOf [
      rdf:type owl:Restriction ;
      owl:allValuesFrom [
          rdf:type owl:Class ;
          owl:unionOf (
              <http://lpis.csd.auth.gr/ontologies/2015/OoSSA.ttl#Avionics>
              <http://lpis.csd.auth.gr/ontologies/2015/OoSSA.ttl#RB>
            ) ;
        ] ;
      owl:onProperty CSSP:hasAbstractionLevel ;
    ] ;
.
CSSP:FDIRRequirement-Handling
  rdf:type owl:Class ;
  rdfs:comment """Avionics level:

RB level: FDIR Requirements describes how a fault / error / failure shall be handled by the OBSW."""^^xsd:string ;
  rdfs:label "FDIRRequirement-Handling"^^xsd:string ;
  rdfs:subClassOf CSSP:FunctionalRequirement ;
  rdfs:subClassOf [
      rdf:type owl:Restriction ;
      owl:allValuesFrom [
          rdf:type owl:Class ;
          owl:unionOf (
              <http://lpis.csd.auth.gr/ontologies/2015/OoSSA.ttl#Avionics>
              <http://lpis.csd.auth.gr/ontologies/2015/OoSSA.ttl#RB>
            ) ;
        ] ;
      owl:onProperty CSSP:hasAbstractionLevel ;
    ] ;
.
CSSP:FDIRRequirements-Recovery
  rdf:type owl:Class ;
  rdfs:comment """Avionics level: FDIR requirements at avionics level are mostly addressed in a separate FDIR specification. The following represent a recovery requirement performed by the Reconfiguration Module (RM).

RB level: Recovery actions are categorised as FDIR Requirements (Recovery). They are either specified in a standard RB such as the following example."""^^xsd:string ;
  rdfs:label "FDIRRequirements-Recovery"^^xsd:string ;
  rdfs:subClassOf CSSP:FunctionalRequirement ;
  rdfs:subClassOf [
      rdf:type owl:Restriction ;
      owl:allValuesFrom [
          rdf:type owl:Class ;
          owl:unionOf (
              <http://lpis.csd.auth.gr/ontologies/2015/OoSSA.ttl#Avionics>
              <http://lpis.csd.auth.gr/ontologies/2015/OoSSA.ttl#RB>
            ) ;
        ] ;
      owl:onProperty CSSP:hasAbstractionLevel ;
    ] ;
.
CSSP:FDIRSizingRequirement
  rdf:type owl:Class ;
  rdfs:comment "RB level: All requirements that are used to size the maximum perimeter of FDIR-related monitoring and actions are considered as FDIR Sizing Requirements"^^xsd:string ;
  rdfs:label "FDIRSizing requirement"^^xsd:string ;
  rdfs:subClassOf CSSP:PerformanceRequirements ;
  rdfs:subClassOf [
      rdf:type owl:Restriction ;
      owl:allValuesFrom <http://lpis.csd.auth.gr/ontologies/2015/OoSSA.ttl#RB> ;
      owl:onProperty CSSP:hasAbstractionLevel ;
    ] ;
.
CSSP:FunctionInputRequirement
  rdf:type owl:Class ;
  rdfs:comment "RB level: Function Input Requirements declare the input to be used for the function."^^xsd:string ;
  rdfs:label "Function input requirement"^^xsd:string ;
  rdfs:subClassOf CSSP:FunctionalRequirement ;
  rdfs:subClassOf [
      rdf:type owl:Restriction ;
      owl:allValuesFrom <http://lpis.csd.auth.gr/ontologies/2015/OoSSA.ttl#RB> ;
      owl:onProperty CSSP:hasAbstractionLevel ;
    ] ;
.
CSSP:FunctionModeDefinitionRequirement
  rdf:type owl:Class ;
  rdfs:comment "RB level: A Function Mode Definition Requirement specifies different functional modes that shall be supported by the function."^^xsd:string ;
  rdfs:label "Function mode definition requirement"^^xsd:string ;
  rdfs:subClassOf CSSP:FunctionalRequirement ;
  rdfs:subClassOf [
      rdf:type owl:Restriction ;
      owl:allValuesFrom <http://lpis.csd.auth.gr/ontologies/2015/OoSSA.ttl#RB> ;
      owl:onProperty CSSP:hasAbstractionLevel ;
    ] ;
.
CSSP:FunctionModeInitialisationRequirement
  rdf:type owl:Class ;
  rdfs:comment "RB level: A Function Mode Initialisation Requirement specifies the applicable mode upon initialisation of the function."^^xsd:string ;
  rdfs:label "Function mode initialisation requirement"^^xsd:string ;
  rdfs:subClassOf CSSP:FunctionalRequirement ;
  rdfs:subClassOf [
      rdf:type owl:Restriction ;
      owl:allValuesFrom <http://lpis.csd.auth.gr/ontologies/2015/OoSSA.ttl#RB> ;
      owl:onProperty CSSP:hasAbstractionLevel ;
    ] ;
.
CSSP:FunctionModeTransitionRequirement
  rdf:type owl:Class ;
  rdfs:comment "RB level: A Function Mode transition represent the passage from a function mode to another."^^xsd:string ;
  rdfs:label "Function mode transition requirement"^^xsd:string ;
  rdfs:subClassOf CSSP:FunctionalRequirement ;
  rdfs:subClassOf [
      rdf:type owl:Restriction ;
      owl:allValuesFrom <http://lpis.csd.auth.gr/ontologies/2015/OoSSA.ttl#RB> ;
      owl:onProperty CSSP:hasAbstractionLevel ;
    ] ;
.
CSSP:FunctionalCapabilityRequirement
  rdf:type owl:Class ;
  rdfs:comment """Avionics level: Functional capability requirements specifies functionalities to be provided either by the avionics system as a whole, or by a subsystem, or by one unit of a subsystem.

RB level: A functional capability requirements expresses what the function is expected to do or perform. Several forms and styles of requirements are possible."""^^xsd:string ;
  rdfs:label "Functional capability requirement"^^xsd:string ;
  rdfs:subClassOf CSSP:FunctionalRequirement ;
  rdfs:subClassOf [
      rdf:type owl:Restriction ;
      owl:allValuesFrom [
          rdf:type owl:Class ;
          owl:unionOf (
              <http://lpis.csd.auth.gr/ontologies/2015/OoSSA.ttl#Avionics>
              <http://lpis.csd.auth.gr/ontologies/2015/OoSSA.ttl#RB>
            ) ;
        ] ;
      owl:onProperty CSSP:hasAbstractionLevel ;
    ] ;
.
CSSP:FunctionalProperty
  rdf:type owl:Class ;
  rdfs:subClassOf CSSP:Property ;
.
CSSP:FunctionalRequirement
  rdf:type owl:Class ;
  rdfs:comment """System spacecraft level: functional requirements define what the system shall perform, in order to conform to the needs / mission statement or requirements of the user.

Avionics level: Avionics functional requirements gather either requirements that are valid across the whole avionics, or functional requirements of a given avionics unit.

RB level: Functional requirements express the expected capabilities of the software system in terms of supported functionalities, algorithm and protocols, mode definitions and initialisation. They are broken down in several sub-categories as it follows."""^^xsd:string ;
  rdfs:label "Functional requirement"^^xsd:string ;
  rdfs:subClassOf CSSP:Requirement ;
  rdfs:subClassOf [
      rdf:type owl:Restriction ;
      owl:allValuesFrom [
          rdf:type owl:Class ;
          owl:unionOf (
              <http://lpis.csd.auth.gr/ontologies/2015/OoSSA.ttl#SystemSpacecraft>
              <http://lpis.csd.auth.gr/ontologies/2015/OoSSA.ttl#Avionics>
              <http://lpis.csd.auth.gr/ontologies/2015/OoSSA.ttl#RB>
              <http://lpis.csd.auth.gr/ontologies/2015/OoSSA.ttl#TS>
            ) ;
        ] ;
      owl:onProperty CSSP:hasAbstractionLevel ;
    ] ;
.
CSSP:FunctionalSoftwareRequirement
  rdf:type owl:Class ;
  rdfs:comment "System spacecraft level: These requirements prescribe an expected high-level OBSW functionality."^^xsd:string ;
  rdfs:label "Functional software requirement"^^xsd:string ;
  rdfs:subClassOf CSSP:OnBoardSoftwareRequirement ;
  rdfs:subClassOf [
      rdf:type owl:Restriction ;
      owl:allValuesFrom <http://lpis.csd.auth.gr/ontologies/2015/OoSSA.ttl#SystemSpacecraft> ;
      owl:onProperty CSSP:hasAbstractionLevel ;
    ] ;
.
CSSP:InterfaceRequirement
  rdf:type owl:Class ;
  rdfs:comment "RB level: Interface Requirements gather all requirement related to how the OBSW interfaces with the rest of the avionics and vice versa."^^xsd:string ;
  rdfs:label "Interface requirement"^^xsd:string ;
  rdfs:subClassOf CSSP:Requirement ;
  rdfs:subClassOf [
      rdf:type owl:Restriction ;
      owl:allValuesFrom [
          rdf:type owl:Class ;
          owl:unionOf (
              <http://lpis.csd.auth.gr/ontologies/2015/OoSSA.ttl#RB>
              <http://lpis.csd.auth.gr/ontologies/2015/OoSSA.ttl#TS>
            ) ;
        ] ;
      owl:onProperty CSSP:hasAbstractionLevel ;
    ] ;
.
CSSP:MemoryStorageRequirement
  rdf:type owl:Class ;
  rdfs:comment "RB level: Memory storage requirements describe an amount of space that shall be used in memory to store some software elements."^^xsd:string ;
  rdfs:label "Memory storage requirement"^^xsd:string ;
  rdfs:subClassOf CSSP:StoragePerformanceRequirements ;
  rdfs:subClassOf [
      rdf:type owl:Restriction ;
      owl:allValuesFrom <http://lpis.csd.auth.gr/ontologies/2015/OoSSA.ttl#RB> ;
      owl:onProperty CSSP:hasAbstractionLevel ;
    ] ;
.
CSSP:MissionRequirement
  rdf:type owl:Class ;
  rdfs:comment """System spacecraft level: Mission requirements are requirements that are directly induced by the mission scenario. A sizeable part of them could be considered as a specialized category of functional requirements.
However, in the general case those requirements may encompass a combination of functional and performance requirements.
For this reason, we prefer to keep them in a separate category.
It is worth to notice that: (i) this class of requirements is applicable only at system level; (ii) it is
not obvious to single out example of requirements in this category for which there could be a
flow-down down to the software level."""^^xsd:string ;
  rdfs:label "Mission requirement"^^xsd:string ;
  rdfs:subClassOf CSSP:Requirement ;
  rdfs:subClassOf [
      rdf:type owl:Restriction ;
      owl:allValuesFrom <http://lpis.csd.auth.gr/ontologies/2015/OoSSA.ttl#SystemSpacecraft> ;
      owl:onProperty CSSP:hasAbstractionLevel ;
    ] ;
.
CSSP:MissionisationRequirement
  rdf:type owl:Class ;
  rdfs:comment "RB level: Missionization requirements describe which elements shall be considered as “missionizable” (i.e., whose values are determined only with an input from the spacecraft data base)."^^xsd:string ;
  rdfs:label "Missionisation requirement"^^xsd:string ;
  rdfs:subClassOf CSSP:DesignAndConstructionRequirement ;
  rdfs:subClassOf [
      rdf:type owl:Restriction ;
      owl:allValuesFrom <http://lpis.csd.auth.gr/ontologies/2015/OoSSA.ttl#RB> ;
      owl:onProperty CSSP:hasAbstractionLevel ;
    ] ;
.
CSSP:ModeDefinitionRequirement
  rdf:type owl:Class ;
  rdfs:comment """System spacecraft level: Mode definition requirements defines modes at spacecraft level and expected behavior in those modes.

Avionics level: Mode Definition Requirements state the different modes for a subsystem or a unit. This is the full range of status applicable to an equipment unit, rather than its view from a client application (for example the GNC)."""^^xsd:string ;
  rdfs:label "Mode definition requirement"^^xsd:string ;
  rdfs:subClassOf CSSP:FunctionalRequirement ;
  rdfs:subClassOf [
      rdf:type owl:Restriction ;
      owl:allValuesFrom [
          rdf:type owl:Class ;
          owl:unionOf (
              <http://lpis.csd.auth.gr/ontologies/2015/OoSSA.ttl#SystemSpacecraft>
              <http://lpis.csd.auth.gr/ontologies/2015/OoSSA.ttl#Avionics>
            ) ;
        ] ;
      owl:onProperty CSSP:hasAbstractionLevel ;
    ] ;
.
CSSP:ModeTransitionRequirement
  rdf:type owl:Class ;
  rdfs:comment """System spacecraft level: Mode Transition Requirements describes how changes of mode are triggered. A change of mode is typically either autonomous or subject to a ground command.

Avionics level: Mode Transition requirements specifies either generic capabilities for mode transitions, or how a transition from a mode to another shall occur."""^^xsd:string ;
  rdfs:label "Mode transition requirement"^^xsd:string ;
  rdfs:subClassOf CSSP:FunctionalRequirement ;
  rdfs:subClassOf [
      rdf:type owl:Restriction ;
      owl:allValuesFrom [
          rdf:type owl:Class ;
          owl:unionOf (
              <http://lpis.csd.auth.gr/ontologies/2015/OoSSA.ttl#SystemSpacecraft>
              <http://lpis.csd.auth.gr/ontologies/2015/OoSSA.ttl#Avionics>
            ) ;
        ] ;
      owl:onProperty CSSP:hasAbstractionLevel ;
    ] ;
.
CSSP:NonFunctionalProperty
  rdf:type owl:Class ;
  rdfs:subClassOf CSSP:Property ;
.
CSSP:NumericalPrecisionRequirement
  rdf:type owl:Class ;
  rdfs:comment "RB level: Numerical Precision Requirements specify the degree of numerical precision required for a given processing activity."^^xsd:string ;
  rdfs:label "Numerical precision requirement"^^xsd:string ;
  rdfs:subClassOf CSSP:DesignAndConstructionRequirement ;
  rdfs:subClassOf [
      rdf:type owl:Restriction ;
      owl:allValuesFrom <http://lpis.csd.auth.gr/ontologies/2015/OoSSA.ttl#RB> ;
      owl:onProperty CSSP:hasAbstractionLevel ;
    ] ;
.
CSSP:OBSW-OperationRequirement
  rdf:type owl:Class ;
  rdfs:comment "System spacecraft level: These requirements specify how the OBSW is expected to be used by an operator."^^xsd:string ;
  rdfs:label "OBSW-Operation requirement"^^xsd:string ;
  rdfs:subClassOf CSSP:OnBoardSoftwareRequirement ;
  rdfs:subClassOf [
      rdf:type owl:Restriction ;
      owl:allValuesFrom <http://lpis.csd.auth.gr/ontologies/2015/OoSSA.ttl#SystemSpacecraft> ;
      owl:onProperty CSSP:hasAbstractionLevel ;
    ] ;
.
CSSP:OBSWInitialisationPerformanceRequirement
  rdf:type owl:Class ;
  rdfs:comment """Avionics level: OBSW initialisation Performance Requirements specifies initialisation requirements specific to the OBSW. They are therefore gathered in a separate category.

RB level: OBSW Initialisation Performance Requirements constraints the conditions for the start and initialisation of the OBSW."""^^xsd:string ;
  rdfs:label "OBSWInitialisation performance requirement"^^xsd:string ;
  rdfs:subClassOf CSSP:PerformanceRequirements ;
  rdfs:subClassOf [
      rdf:type owl:Restriction ;
      owl:allValuesFrom [
          rdf:type owl:Class ;
          owl:unionOf (
              <http://lpis.csd.auth.gr/ontologies/2015/OoSSA.ttl#Avionics>
              <http://lpis.csd.auth.gr/ontologies/2015/OoSSA.ttl#RB>
            ) ;
        ] ;
      owl:onProperty CSSP:hasAbstractionLevel ;
    ] ;
.
CSSP:OBSWRebootPerformanceRequirements
  rdf:type owl:Class ;
  rdfs:comment "Avionics level: OBSW reboot performance include timing constraints on the performance of the on-board software reboot. This requirement would then apply to the boot software rather than the central software."^^xsd:string ;
  rdfs:label "OBSWReboot performance requirements"^^xsd:string ;
  rdfs:subClassOf CSSP:PerformanceRequirements ;
  rdfs:subClassOf [
      rdf:type owl:Restriction ;
      owl:allValuesFrom <http://lpis.csd.auth.gr/ontologies/2015/OoSSA.ttl#Avionics> ;
      owl:onProperty CSSP:hasAbstractionLevel ;
    ] ;
.
CSSP:ObservabilityRequirement
  rdf:type owl:Class ;
  rdfs:comment "RB level: Observability Requirements describe how the execution or the result processed by a given function or the OBSW as a whole can be observed from an external system (typically the ground)."^^xsd:string ;
  rdfs:label "Observability requirement"^^xsd:string ;
  rdfs:subClassOf CSSP:InterfaceRequirement ;
  rdfs:subClassOf [
      rdf:type owl:Restriction ;
      owl:allValuesFrom <http://lpis.csd.auth.gr/ontologies/2015/OoSSA.ttl#RB> ;
      owl:onProperty CSSP:hasAbstractionLevel ;
    ] ;
.
CSSP:ObservabilityRequirements
  rdf:type owl:Class ;
  rdfs:comment "Avionics level: Observability requirements specifies the observable perimeter for the avionics system."^^xsd:string ;
  rdfs:label "Observability requirements"^^xsd:string ;
  rdfs:subClassOf CSSP:FunctionalRequirement ;
  rdfs:subClassOf [
      rdf:type owl:Restriction ;
      owl:allValuesFrom <http://lpis.csd.auth.gr/ontologies/2015/OoSSA.ttl#Avionics> ;
      owl:onProperty CSSP:hasAbstractionLevel ;
    ] ;
.
CSSP:On-boardSoftwareRequirement
  rdf:type owl:Class ;
  rdfs:comment "Avionics level: The most important sub-category regards the OBSW, and gathers requirements on either the OBSW development process or on specific aspects of its implementation."^^xsd:string ;
  rdfs:label "On-board software requirement"^^xsd:string ;
  rdfs:subClassOf CSSP:DesignAndConstructionRequirement ;
  rdfs:subClassOf [
      rdf:type owl:Restriction ;
      owl:allValuesFrom <http://lpis.csd.auth.gr/ontologies/2015/OoSSA.ttl#Avionics> ;
      owl:onProperty CSSP:hasAbstractionLevel ;
    ] ;
.
CSSP:On-boardTCreleaseRequirement
  rdf:type owl:Class ;
  rdfs:comment "RB level: A particular sub-category of performance requirements are those related to on-board TC release, which are typical for automation services such as the Mission Time Line (MTL) or the Orbit Position Scheduler (OPS)."^^xsd:string ;
  rdfs:label "On-board TCrelease requirement"^^xsd:string ;
  rdfs:subClassOf CSSP:PerformanceRequirements ;
  rdfs:subClassOf [
      rdf:type owl:Restriction ;
      owl:allValuesFrom <http://lpis.csd.auth.gr/ontologies/2015/OoSSA.ttl#RB> ;
      owl:onProperty CSSP:hasAbstractionLevel ;
    ] ;
.
CSSP:OnBoardSoftwareRequirement
  rdf:type owl:Class ;
  rdfs:comment "System spacecraft level: Requirements for On-board Software at spacecraft level are typically process oriented (adherence to standards, or use of a given testing strategy)."^^xsd:string ;
  rdfs:label "On board software requirement"^^xsd:string ;
  rdfs:subClassOf CSSP:Requirement ;
  rdfs:subClassOf [
      rdf:type owl:Restriction ;
      owl:allValuesFrom <http://lpis.csd.auth.gr/ontologies/2015/OoSSA.ttl#SystemSpacecraft> ;
      owl:onProperty CSSP:hasAbstractionLevel ;
    ] ;
.
CSSP:OperabilityRequirement
  rdf:type owl:Class ;
  rdfs:comment "RB level: The expected operability of functions or units is described in Operability Requirements."^^xsd:string ;
  rdfs:label "Operability requirement"^^xsd:string ;
  rdfs:subClassOf CSSP:OperationRequirement ;
  rdfs:subClassOf [
      rdf:type owl:Restriction ;
      owl:allValuesFrom <http://lpis.csd.auth.gr/ontologies/2015/OoSSA.ttl#RB> ;
      owl:onProperty CSSP:hasAbstractionLevel ;
    ] ;
.
CSSP:OperationRequirement
  rdf:type owl:Class ;
  rdfs:comment """System spacecraft level: Operational Requirements comprise requirement related to how to correctly operate the spacecraft or how the spacecraft is expected to be operated.

Avionics level: Operation requirements are related to how functions of the avionics or of a unit are operated or are expected to behave or relate to other functions."""^^xsd:string ;
  rdfs:label "Operational requirement"^^xsd:string ;
  rdfs:subClassOf CSSP:Requirement ;
  rdfs:subClassOf [
      rdf:type owl:Restriction ;
      owl:allValuesFrom [
          rdf:type owl:Class ;
          owl:unionOf (
              <http://lpis.csd.auth.gr/ontologies/2015/OoSSA.ttl#SystemSpacecraft>
              <http://lpis.csd.auth.gr/ontologies/2015/OoSSA.ttl#Avionics>
              <http://lpis.csd.auth.gr/ontologies/2015/OoSSA.ttl#RB>
              <http://lpis.csd.auth.gr/ontologies/2015/OoSSA.ttl#TS>
            ) ;
        ] ;
      owl:onProperty CSSP:hasAbstractionLevel ;
    ] ;
.
CSSP:PAandRAMSRequirements
  rdf:type owl:Class ;
  rdfs:comment """Avionics level: PA & RAMS Requirements at avionics level typically comprise requirements related to the safety of operation of equipment.
Most are related to secure safeguards for the manipulation of equipment or to prevent hazardous activation of equipment on ground (e.g., antenna emissions).
Physical barriers are considered out of scope.
Electrical barriers could be interesting."""^^xsd:string ;
  rdfs:label "PAand RAMSRequirements"^^xsd:string ;
  rdfs:subClassOf CSSP:Requirement ;
  rdfs:subClassOf [
      rdf:type owl:Restriction ;
      owl:allValuesFrom [
          rdf:type owl:Class ;
          owl:unionOf (
              <http://lpis.csd.auth.gr/ontologies/2015/OoSSA.ttl#Avionics>
              <http://lpis.csd.auth.gr/ontologies/2015/OoSSA.ttl#TS>
            ) ;
        ] ;
      owl:onProperty CSSP:hasAbstractionLevel ;
    ] ;
.
CSSP:PatchRequirement
  rdf:type owl:Class ;
  rdfs:comment "Avionics level: Patch requirements are a specific sub-category of functional requirements related to all functional needs to support patch of the OBSW. Please note that at avionics level, requirements relate to the Data Handling System as a whole."^^xsd:string ;
  rdfs:label "Patch requirement"^^xsd:string ;
  rdfs:subClassOf CSSP:FunctionalRequirement ;
  rdfs:subClassOf [
      rdf:type owl:Restriction ;
      owl:allValuesFrom <http://lpis.csd.auth.gr/ontologies/2015/OoSSA.ttl#Avionics> ;
      owl:onProperty CSSP:hasAbstractionLevel ;
    ] ;
.
CSSP:PatchStorageRequirement
  rdf:type owl:Class ;
  rdfs:comment "RB level: Patch storage requirements describe an amount of space that shall be used in memory to store patches. This is singled out as a dedicated class, as patches are software elements not related to the current configuration and have a particular treatment in the lifecycle of the spacecraft."^^xsd:string ;
  rdfs:label "Patch storage requirement"^^xsd:string ;
  rdfs:subClassOf CSSP:StoragePerformanceRequirements ;
  rdfs:subClassOf [
      rdf:type owl:Restriction ;
      owl:allValuesFrom <http://lpis.csd.auth.gr/ontologies/2015/OoSSA.ttl#RB> ;
      owl:onProperty CSSP:hasAbstractionLevel ;
    ] ;
.
CSSP:PerformanceRequirements
  rdf:type owl:Class ;
  rdfs:comment """Avionics level:

RB level: Performance requirements impose either constraints on the execution of functions or expected performances."""^^xsd:string ;
  rdfs:label "Performance requirements"^^xsd:string ;
  rdfs:subClassOf CSSP:Requirement ;
  rdfs:subClassOf [
      rdf:type owl:Restriction ;
      owl:allValuesFrom [
          rdf:type owl:Class ;
          owl:unionOf (
              <http://lpis.csd.auth.gr/ontologies/2015/OoSSA.ttl#Avionics>
              <http://lpis.csd.auth.gr/ontologies/2015/OoSSA.ttl#RB>
              <http://lpis.csd.auth.gr/ontologies/2015/OoSSA.ttl#TS>
            ) ;
        ] ;
      owl:onProperty CSSP:hasAbstractionLevel ;
    ] ;
.
CSSP:PrecedenceConstraintsonFunctionalCapabilityRequirement
  rdf:type owl:Class ;
  rdfs:comment "RB level: Precedence Constraints on Functional Capability Requirements specifies how a function is the presence of multiple requests or occurrences of its expected processing."^^xsd:string ;
  rdfs:label "Precedence constraintson functional capability requirement"^^xsd:string ;
  rdfs:subClassOf CSSP:FunctionalRequirement ;
  rdfs:subClassOf [
      rdf:type owl:Restriction ;
      owl:allValuesFrom <http://lpis.csd.auth.gr/ontologies/2015/OoSSA.ttl#RB> ;
      owl:onProperty CSSP:hasAbstractionLevel ;
    ] ;
.
CSSP:ProcessingInputAvailability
  rdf:type owl:Class ;
  rdfs:comment "RB level: Processing Input Availability Requirements imposes constraints on the availability of input data to start a processing activity."^^xsd:string ;
  rdfs:label "Processing input availability"^^xsd:string ;
  rdfs:subClassOf CSSP:PerformanceRequirements ;
  rdfs:subClassOf [
      rdf:type owl:Restriction ;
      owl:allValuesFrom <http://lpis.csd.auth.gr/ontologies/2015/OoSSA.ttl#RB> ;
      owl:onProperty CSSP:hasAbstractionLevel ;
    ] ;
.
CSSP:ProcessingPrecedenceConstraintRequirement
  rdf:type owl:Class ;
  rdfs:comment "RB level: Processing Precedence Constraint requirements express performance expectations in terms of completion of a given processing in a before the occurrence of an event."^^xsd:string ;
  rdfs:label "Processing precedence constraint requirement"^^xsd:string ;
  rdfs:subClassOf CSSP:PerformanceRequirements ;
  rdfs:subClassOf [
      rdf:type owl:Restriction ;
      owl:allValuesFrom <http://lpis.csd.auth.gr/ontologies/2015/OoSSA.ttl#RB> ;
      owl:onProperty CSSP:hasAbstractionLevel ;
    ] ;
.
CSSP:ProcessingResultsRequirement
  rdf:type owl:Class ;
  rdfs:comment "RB level: Processing result requirements describe expectations on the result of a processing activity."^^xsd:string ;
  rdfs:label "Processing results requirement"^^xsd:string ;
  rdfs:subClassOf CSSP:PerformanceRequirements ;
  rdfs:subClassOf [
      rdf:type owl:Restriction ;
      owl:allValuesFrom <http://lpis.csd.auth.gr/ontologies/2015/OoSSA.ttl#RB> ;
      owl:onProperty CSSP:hasAbstractionLevel ;
    ] ;
.
CSSP:ProcessingTimingRequirement
  rdf:type owl:Class ;
  rdfs:comment "RB level: Processing timing requirements typically express performance expectations in terms of completion of a given processing in a given time window. It should be noted that this could be considered as a specialization of the previous category."^^xsd:string ;
  rdfs:label "Processing timing requirement"^^xsd:string ;
  rdfs:subClassOf CSSP:PerformanceRequirements ;
  rdfs:subClassOf [
      rdf:type owl:Restriction ;
      owl:allValuesFrom <http://lpis.csd.auth.gr/ontologies/2015/OoSSA.ttl#RB> ;
      owl:onProperty CSSP:hasAbstractionLevel ;
    ] ;
.
CSSP:Property
  rdf:type owl:Class ;
  rdfs:subClassOf <http://lpis.csd.auth.gr/ontologies/2015/OoSSA.ttl#Characteristic> ;
  owl:equivalentClass <http://lpis.csd.auth.gr/ontologies/2015/PRP#PropertyPattern> ;
.
CSSP:ProtocolRequirement
  rdf:type owl:Class ;
  rdfs:comment "Avionics level: Protocol requirements specify a given protocol that shall be implemented by the avionics, a subsystem or an avionics unit. We distinguish protocol requirements from functional capabilities, as they specify expected behaviour or fundamental characteristic of the expected behaviour."^^xsd:string ;
  rdfs:label "Protocol requirement"^^xsd:string ;
  rdfs:subClassOf CSSP:FunctionalRequirement ;
  rdfs:subClassOf [
      rdf:type owl:Restriction ;
      owl:allValuesFrom <http://lpis.csd.auth.gr/ontologies/2015/OoSSA.ttl#Avionics> ;
      owl:onProperty CSSP:hasAbstractionLevel ;
    ] ;
.
CSSP:RedundancyΑndCross-StrappingRequirement
  rdf:type owl:Class ;
  rdfs:comment "Avionics level:"^^xsd:string ;
  rdfs:label "Redundancy αnd cross-Strapping requirement"^^xsd:string ;
  rdfs:subClassOf CSSP:AvionicsTopologyRequirement ;
  rdfs:subClassOf [
      rdf:type owl:Restriction ;
      owl:allValuesFrom <http://lpis.csd.auth.gr/ontologies/2015/OoSSA.ttl#Avionics> ;
      owl:onProperty CSSP:hasAbstractionLevel ;
    ] ;
.
CSSP:RelativeTimeWindowRequirement
  rdf:type owl:Class ;
  rdfs:comment "RB level: This category comprises requirements that prescribes a given relative time window to perform a given acquisition or a processing activity."^^xsd:string ;
  rdfs:label "Relative time window requirement"^^xsd:string ;
  rdfs:subClassOf CSSP:PerformanceRequirements ;
  rdfs:subClassOf [
      rdf:type owl:Restriction ;
      owl:allValuesFrom <http://lpis.csd.auth.gr/ontologies/2015/OoSSA.ttl#RB> ;
      owl:onProperty CSSP:hasAbstractionLevel ;
    ] ;
.
CSSP:RepresentationRequirement
  rdf:type owl:Class ;
  rdfs:comment "Avionics level: These requirements impose a given representation format for some elements."^^xsd:string ;
  rdfs:label "Representation requirement"^^xsd:string ;
  rdfs:subClassOf CSSP:DesignAndConstructionRequirement ;
  rdfs:subClassOf [
      rdf:type owl:Restriction ;
      owl:allValuesFrom <http://lpis.csd.auth.gr/ontologies/2015/OoSSA.ttl#Avionics> ;
      owl:onProperty CSSP:hasAbstractionLevel ;
    ] ;
.
CSSP:Requirement
  rdf:type owl:Class ;
  spin:rule [
      rdf:type sp:Construct ;
      sp:templates (
          [
            sp:object CSSP:AbstractRequirement ;
            sp:predicate rdf:type ;
            sp:subject spin:_this ;
          ]
        ) ;
      sp:where (
          [
            sp:object [
                sp:varName "x"^^xsd:string ;
              ] ;
            sp:predicate CSSP:hasClause ;
            sp:subject spin:_this ;
          ]
          [
            rdf:type sp:TriplePath ;
            sp:object [
                sp:varName "e"^^xsd:string ;
              ] ;
            sp:path [
                rdf:type sp:ModPath ;
                sp:modMax -2 ;
                sp:modMin 1 ;
                sp:subPath <http://lpis.csd.auth.gr/ontologies/2015/RBLP#isRelatedToAttribute> ;
              ] ;
            sp:subject [
                sp:varName "x"^^xsd:string ;
              ] ;
          ]
          [
            sp:object owl:Class ;
            sp:predicate rdf:type ;
            sp:subject [
                sp:varName "e"^^xsd:string ;
              ] ;
          ]
        ) ;
    ] ;
  spin:rule [
      rdf:type sp:Construct ;
      sp:templates (
          [
            sp:object spin:_this ;
            sp:predicate CSSP:hasRequirement ;
            sp:subject [
                sp:varName "e"^^xsd:string ;
              ] ;
          ]
        ) ;
      sp:where (
          [
            sp:object [
                sp:varName "x"^^xsd:string ;
              ] ;
            sp:predicate CSSP:hasClause ;
            sp:subject spin:_this ;
          ]
          [
            rdf:type sp:TriplePath ;
            sp:object [
                sp:varName "e"^^xsd:string ;
              ] ;
            sp:path [
                rdf:type sp:ModPath ;
                sp:modMax -2 ;
                sp:modMin 1 ;
                sp:subPath <http://lpis.csd.auth.gr/ontologies/2015/RBLP#isRelatedToAttribute> ;
              ] ;
            sp:subject [
                sp:varName "x"^^xsd:string ;
              ] ;
          ]
          [
            sp:object <http://lpis.csd.auth.gr/ontologies/2015/RBLP#Entity> ;
            sp:predicate rdf:type ;
            sp:subject [
                sp:varName "e"^^xsd:string ;
              ] ;
          ]
        ) ;
    ] ;
  spin:rule [
      rdf:type sp:Construct ;
      sp:templates (
          [
            sp:object spin:_this ;
            sp:predicate CSSP:isSubjectofRequirement ;
            sp:subject [
                sp:varName "e"^^xsd:string ;
              ] ;
          ]
        ) ;
      sp:where (
          [
            sp:object [
                sp:varName "x"^^xsd:string ;
              ] ;
            sp:predicate CSSP:hasMain ;
            sp:subject spin:_this ;
          ]
          [
            sp:object [
                sp:varName "e"^^xsd:string ;
              ] ;
            sp:predicate <http://lpis.csd.auth.gr/ontologies/2015/RBLP#isRelatedToSubject> ;
            sp:subject [
                sp:varName "x"^^xsd:string ;
              ] ;
          ]
          [
            sp:object <http://lpis.csd.auth.gr/ontologies/2015/RBLP#SimpleEntity> ;
            sp:predicate rdf:type ;
            sp:subject [
                sp:varName "e"^^xsd:string ;
              ] ;
          ]
        ) ;
    ] ;
  rdfs:subClassOf <http://lpis.csd.auth.gr/ontologies/2015/OoSSA.ttl#Characteristic> ;
.
CSSP:ReusePotentialRequirement
  rdf:type owl:Class ;
  rdfs:comment "RB level: Reuse potential requirements impose implementation constraints to foster the reuse potential of the software."^^xsd:string ;
  rdfs:label "Reuse potential requirement"^^xsd:string ;
  rdfs:subClassOf CSSP:DesignAndConstructionRequirement ;
  rdfs:subClassOf [
      rdf:type owl:Restriction ;
      owl:allValuesFrom <http://lpis.csd.auth.gr/ontologies/2015/OoSSA.ttl#RB> ;
      owl:onProperty CSSP:hasAbstractionLevel ;
    ] ;
.
CSSP:RobustnessRequirement
  rdf:type owl:Class ;
  rdfs:comment "RB level: Robustness requirements describe implementation constraints imposed to foster robustness of the software."^^xsd:string ;
  rdfs:label "Robustness requirement"^^xsd:string ;
  rdfs:subClassOf CSSP:DesignAndConstructionRequirement ;
  rdfs:subClassOf [
      rdf:type owl:Restriction ;
      owl:allValuesFrom <http://lpis.csd.auth.gr/ontologies/2015/OoSSA.ttl#RB> ;
      owl:onProperty CSSP:hasAbstractionLevel ;
    ] ;
.
CSSP:StorageAverageDataRateRequirement
  rdf:type owl:Class ;
  rdfs:comment "RB level: Storage average data rate requirements describe the average data rate to be sustained by a function or the OBSW."^^xsd:string ;
  rdfs:label "Storage average data rate requirement"^^xsd:string ;
  rdfs:subClassOf CSSP:StoragePerformanceRequirements ;
  rdfs:subClassOf [
      rdf:type owl:Restriction ;
      owl:allValuesFrom <http://lpis.csd.auth.gr/ontologies/2015/OoSSA.ttl#RB> ;
      owl:onProperty CSSP:hasAbstractionLevel ;
    ] ;
.
CSSP:StorageIntegrityRequirement
  rdf:type owl:Class ;
  rdfs:comment "RB level: Storage Integrity Requirements prescribe how the integrity of a given stored information is checked."^^xsd:string ;
  rdfs:label "Storage integrity requirement"^^xsd:string ;
  rdfs:subClassOf CSSP:StoragePerformanceRequirements ;
  rdfs:subClassOf [
      rdf:type owl:Restriction ;
      owl:allValuesFrom <http://lpis.csd.auth.gr/ontologies/2015/OoSSA.ttl#RB> ;
      owl:onProperty CSSP:hasAbstractionLevel ;
    ] ;
.
CSSP:StorageMaximumDataRateRequirement
  rdf:type owl:Class ;
  rdfs:comment "RB level: Storage maximum data rate requirements describe the maximum data rate to be sustained by a function or the OBSW."^^xsd:string ;
  rdfs:label "Storage maximum data rate requirement"^^xsd:string ;
  rdfs:subClassOf CSSP:StoragePerformanceRequirements ;
  rdfs:subClassOf [
      rdf:type owl:Restriction ;
      owl:allValuesFrom <http://lpis.csd.auth.gr/ontologies/2015/OoSSA.ttl#RB> ;
      owl:onProperty CSSP:hasAbstractionLevel ;
    ] ;
.
CSSP:StoragePerformanceRequirements
  rdf:type owl:Class ;
  rdfs:comment """Avionics level: Storage requirements refer to storage requirements of avionics units.

RB level: Storage requirements declares constraint related to storage of data or part of the OBSW."""^^xsd:string ;
  rdfs:label "Storage performance requirements"^^xsd:string ;
  rdfs:subClassOf CSSP:PerformanceRequirements ;
  rdfs:subClassOf [
      rdf:type owl:Restriction ;
      owl:allValuesFrom [
          rdf:type owl:Class ;
          owl:unionOf (
              <http://lpis.csd.auth.gr/ontologies/2015/OoSSA.ttl#Avionics>
              <http://lpis.csd.auth.gr/ontologies/2015/OoSSA.ttl#RB>
            ) ;
        ] ;
      owl:onProperty CSSP:hasAbstractionLevel ;
    ] ;
.
CSSP:Sub-functionInitialisationRequirement
  rdf:type owl:Class ;
  rdfs:comment "RB level: A sub-function initialization requirement specifies the initialization of an inner part or submodule of a parent function."^^xsd:string ;
  rdfs:label "Sub-function initialisation requirement"^^xsd:string ;
  rdfs:subClassOf CSSP:FunctionalRequirement ;
  rdfs:subClassOf [
      rdf:type owl:Restriction ;
      owl:allValuesFrom <http://lpis.csd.auth.gr/ontologies/2015/OoSSA.ttl#RB> ;
      owl:onProperty CSSP:hasAbstractionLevel ;
    ] ;
.
CSSP:Sub-functionendofInitialisationRequirement
  rdf:type owl:Class ;
  rdfs:comment "RB level: A sub-function end of initialization requirement prescribes an action to be performed just at the end of initialization. It could be considered as the “finalization of the initialization”, so as to prepare nominal function execution."^^xsd:string ;
  rdfs:label "Sub-functionendof initialisation requirement"^^xsd:string ;
  rdfs:subClassOf CSSP:FunctionalRequirement ;
  rdfs:subClassOf [
      rdf:type owl:Restriction ;
      owl:allValuesFrom <http://lpis.csd.auth.gr/ontologies/2015/OoSSA.ttl#RB> ;
      owl:onProperty CSSP:hasAbstractionLevel ;
    ] ;
.
CSSP:Subsystem-UnitTimingRequirements
  rdf:type owl:Class ;
  rdfs:comment "Avionics level: Subsystem / Unit Timing Requirements defines timing constraints on expected functionalities."^^xsd:string ;
  rdfs:label "Subsystem-Unit timing requirements"^^xsd:string ;
  rdfs:subClassOf CSSP:PerformanceRequirements ;
  rdfs:subClassOf [
      rdf:type owl:Restriction ;
      owl:allValuesFrom <http://lpis.csd.auth.gr/ontologies/2015/OoSSA.ttl#Avionics> ;
      owl:onProperty CSSP:hasAbstractionLevel ;
    ] ;
.
CSSP:SubsystemandEquipmentAutonomyRequirement
  rdf:type owl:Class ;
  rdfs:comment "Avionics level: Subsystem and equipment autonomy requirements comprise all requirement related to autonomous operations in absence of ground intervention or unavailability of a subsystem."^^xsd:string ;
  rdfs:label "Subsystemand equipment autonomy requirement"^^xsd:string ;
  rdfs:subClassOf CSSP:Requirement ;
  rdfs:subClassOf [
      rdf:type owl:Restriction ;
      owl:allValuesFrom <http://lpis.csd.auth.gr/ontologies/2015/OoSSA.ttl#Avionics> ;
      owl:onProperty CSSP:hasAbstractionLevel ;
    ] ;
.
CSSP:SubsystemandEquipmentObservabilityRequirement
  rdf:type owl:Class ;
  rdfs:comment """Avionics level: This class of requirements gather requirements on the observability of the avionics subsystem or units.
From the point of view of the avionics specification, these requirements are considered as design requirements."""^^xsd:string ;
  rdfs:label "Subsystemand equipment observability requirement"^^xsd:string ;
  rdfs:subClassOf CSSP:DesignAndConstructionRequirement ;
  rdfs:subClassOf [
      rdf:type owl:Restriction ;
      owl:allValuesFrom <http://lpis.csd.auth.gr/ontologies/2015/OoSSA.ttl#Avionics> ;
      owl:onProperty CSSP:hasAbstractionLevel ;
    ] ;
.
CSSP:SupportRequirement
  rdf:type owl:Class ;
  rdfs:subClassOf CSSP:Requirement ;
  rdfs:subClassOf [
      rdf:type owl:Restriction ;
      owl:allValuesFrom <http://lpis.csd.auth.gr/ontologies/2015/OoSSA.ttl#TS> ;
      owl:onProperty CSSP:hasAbstractionLevel ;
    ] ;
.
CSSP:SynchronizationRequirement
  rdf:type owl:Class ;
  rdfs:comment "Avionics level: Synchronization Requirements specifies synchronization constraints that applies on the avionics or units of the avionics."^^xsd:string ;
  rdfs:label "Synchronization requirement"^^xsd:string ;
  rdfs:subClassOf CSSP:FunctionalRequirement ;
  rdfs:subClassOf [
      rdf:type owl:Restriction ;
      owl:allValuesFrom <http://lpis.csd.auth.gr/ontologies/2015/OoSSA.ttl#Avionics> ;
      owl:onProperty CSSP:hasAbstractionLevel ;
    ] ;
.
CSSP:TCReleaseandAccuracyRequirement
  rdf:type owl:Class ;
  rdfs:comment "Avionics level: TC Release and Accuracy Requirements are a separate category of requirements that describes expectation on the number of TCs that shall be released by the data handling subsystem."^^xsd:string ;
  rdfs:label "TCReleaseand accuracy requirement"^^xsd:string ;
  rdfs:subClassOf CSSP:PerformanceRequirements ;
  rdfs:subClassOf [
      rdf:type owl:Restriction ;
      owl:allValuesFrom <http://lpis.csd.auth.gr/ontologies/2015/OoSSA.ttl#Avionics> ;
      owl:onProperty CSSP:hasAbstractionLevel ;
    ] ;
.
CSSP:TMBandwithRequirement
  rdf:type owl:Class ;
  rdfs:comment """Avionics level: TM Bandwidth Requirements describe the expected TM bandwidth that shall be sustained by the subsystem.

RB level: TM Bandwidth Requirements describes expectation on the amount of data to be received and addressed in a given time window."""^^xsd:string ;
  rdfs:label "TMBandwith requirement"^^xsd:string ;
  rdfs:subClassOf CSSP:PerformanceRequirements ;
  rdfs:subClassOf [
      rdf:type owl:Restriction ;
      owl:allValuesFrom [
          rdf:type owl:Class ;
          owl:unionOf (
              <http://lpis.csd.auth.gr/ontologies/2015/OoSSA.ttl#Avionics>
              <http://lpis.csd.auth.gr/ontologies/2015/OoSSA.ttl#RB>
            ) ;
        ] ;
      owl:onProperty CSSP:hasAbstractionLevel ;
    ] ;
.
CSSP:TimedFunctionalCapabilityRequirement
  rdf:type owl:Class ;
  rdfs:comment "RB level: A Timed Functional Capability Requirement expresses an expected functionality linked to a time event. While these requirements could be considered in the same category of Conditional Functional Capability Requirements, we prefer to keep them separate, as the properties that would stem from them will likely require different analysis framework (e.g., a simple state machine LTS vs. a Timed Automata)."^^xsd:string ;
  rdfs:label "Timed functional capability requirement"^^xsd:string ;
  rdfs:subClassOf CSSP:FunctionalRequirement ;
  rdfs:subClassOf [
      rdf:type owl:Restriction ;
      owl:allValuesFrom <http://lpis.csd.auth.gr/ontologies/2015/OoSSA.ttl#RB> ;
      owl:onProperty CSSP:hasAbstractionLevel ;
    ] ;
.
CSSP:UnitInitialisationPerformanceRequirement
  rdf:type owl:Class ;
  rdfs:comment "Avionics level: Unit Initialization Performance Requirements specifies constraints on the initialization of units."^^xsd:string ;
  rdfs:label "Unit initialisation performance requirement"^^xsd:string ;
  rdfs:subClassOf CSSP:PerformanceRequirements ;
  rdfs:subClassOf [
      rdf:type owl:Restriction ;
      owl:allValuesFrom <http://lpis.csd.auth.gr/ontologies/2015/OoSSA.ttl#Avionics> ;
      owl:onProperty CSSP:hasAbstractionLevel ;
    ] ;
.
CSSP:ValidationRequirements
  rdf:type owl:Class ;
  rdfs:subClassOf CSSP:Requirement ;
  rdfs:subClassOf [
      rdf:type owl:Restriction ;
      owl:allValuesFrom <http://lpis.csd.auth.gr/ontologies/2015/OoSSA.ttl#TS> ;
      owl:onProperty CSSP:hasAbstractionLevel ;
    ] ;
.
CSSP:VerificationRequirement
  rdf:type owl:Class ;
  rdfs:subClassOf CSSP:Requirement ;
  rdfs:subClassOf [
      rdf:type owl:Restriction ;
      owl:allValuesFrom <http://lpis.csd.auth.gr/ontologies/2015/OoSSA.ttl#TS> ;
      owl:onProperty CSSP:hasAbstractionLevel ;
    ] ;
.
CSSP:concretizes
  rdf:type owl:ObjectProperty ;
  rdfs:domain CSSP:ConcreteRequirement ;
  rdfs:range CSSP:AbstractRequirement ;
.
CSSP:formalizes
  rdf:type owl:ObjectProperty ;
  rdfs:domain CSSP:Property ;
  rdfs:label "formalizes"^^xsd:string ;
  rdfs:range CSSP:Requirement ;
  owl:inverseOf CSSP:isFormalizedBy ;
.
CSSP:hasAbstractEntity
  rdf:type owl:ObjectProperty ;
  rdfs:domain CSSP:AbstractRequirement ;
.
CSSP:hasAbstractionLevel
  rdf:type owl:ObjectProperty ;
  rdfs:domain CSSP:Requirement ;
  rdfs:range <http://lpis.csd.auth.gr/ontologies/2015/OoSSA.ttl#AbstractionLevel> ;
.
CSSP:hasClause
  rdf:type owl:ObjectProperty ;
  rdfs:domain CSSP:Requirement ;
  rdfs:range <http://lpis.csd.auth.gr/ontologies/2015/RBLP#ReqDescriptor> ;
.
CSSP:hasMain
  rdf:type owl:ObjectProperty ;
  rdfs:range <http://lpis.csd.auth.gr/ontologies/2015/RBLP#Main> ;
  rdfs:subPropertyOf CSSP:hasClause ;
.
CSSP:hasPort
  rdf:type owl:ObjectProperty ;
  rdfs:domain <http://lpis.csd.auth.gr/ontologies/2015/PRP#PortActivation> ;
  rdfs:range <http://lpis.csd.auth.gr/ontologies/2015/OoSSA.ttl#Port> ;
.
CSSP:hasPrefix
  rdf:type owl:ObjectProperty ;
  rdfs:range <http://lpis.csd.auth.gr/ontologies/2015/RBLP#Prefix> ;
  rdfs:subPropertyOf CSSP:hasClause ;
.
CSSP:hasProperty
  rdf:type owl:ObjectProperty ;
  rdfs:domain <http://lpis.csd.auth.gr/ontologies/2015/OoSSA.ttl#SystemEntity> ;
  rdfs:range CSSP:Property ;
.
CSSP:hasPropertyPattern
  rdf:type owl:ObjectProperty ;
  rdfs:domain CSSP:Property ;
  rdfs:label "has property pattern"^^xsd:string ;
  rdfs:range <http://lpis.csd.auth.gr/ontologies/2015/PRP#PropertyPattern> ;
.
CSSP:hasRequirement
  rdf:type owl:ObjectProperty ;
  rdfs:domain <http://lpis.csd.auth.gr/ontologies/2015/RBLP#Entity> ;
  rdfs:range CSSP:Requirement ;
.
CSSP:hasSuffix
  rdf:type owl:ObjectProperty ;
  rdfs:range <http://lpis.csd.auth.gr/ontologies/2015/RBLP#Suffix> ;
  rdfs:subPropertyOf CSSP:hasClause ;
.
CSSP:isClauseOf
  rdf:type owl:ObjectProperty ;
  rdfs:domain <http://lpis.csd.auth.gr/ontologies/2015/RBLP#ReqDescriptor> ;
  rdfs:range CSSP:Requirement ;
.
CSSP:isFormalizedBy
  rdf:type owl:ObjectProperty ;
  rdfs:domain CSSP:Requirement ;
  rdfs:range CSSP:Property ;
.
CSSP:isMainOf
  rdf:type owl:ObjectProperty ;
  rdfs:subPropertyOf CSSP:isClauseOf ;
  owl:inverseOf CSSP:hasMain ;
.
CSSP:isPrefixOf
  rdf:type owl:ObjectProperty ;
  rdfs:range <http://lpis.csd.auth.gr/ontologies/2015/RBLP#ComplexPrefix> ;
  rdfs:subPropertyOf CSSP:isClauseOf ;
  owl:inverseOf CSSP:hasPrefix ;
.
CSSP:isPropertyOf
  rdf:type owl:ObjectProperty ;
  rdfs:domain CSSP:Property ;
  rdfs:range <http://lpis.csd.auth.gr/ontologies/2015/OoSSA.ttl#SystemEntity> ;
  owl:inverseOf CSSP:hasProperty ;
.
CSSP:isRequirementOf
  rdf:type owl:ObjectProperty ;
  rdfs:domain CSSP:Requirement ;
  rdfs:range <http://lpis.csd.auth.gr/ontologies/2015/RBLP#Entity> ;
  owl:inverseOf CSSP:hasRequirement ;
.
CSSP:isSubjectofRequirement
  rdf:type owl:ObjectProperty ;
  rdfs:domain <http://lpis.csd.auth.gr/ontologies/2015/RBLP#SimpleEntity> ;
  rdfs:subPropertyOf CSSP:hasRequirement ;
.
CSSP:isSuffixOf
  rdf:type owl:ObjectProperty ;
  rdfs:range <http://lpis.csd.auth.gr/ontologies/2015/RBLP#ComplexSuffix> ;
  rdfs:subPropertyOf CSSP:isClauseOf ;
  owl:inverseOf CSSP:hasSuffix ;
.
CSSP:mainAbstractEntity
  rdf:type owl:ObjectProperty ;
  rdfs:domain CSSP:AbstractRequirement ;
  rdfs:subPropertyOf CSSP:hasAbstractEntity ;
.
<http://lpis.csd.auth.gr/ontologies/2015/OoSSA.ttl#AbstractionLevel>
  rdf:type owl:Class ;
  rdfs:subClassOf <http://lpis.csd.auth.gr/ontologies/2015/OoSSA.ttl#Characteristic> ;
.
<http://lpis.csd.auth.gr/ontologies/2015/OoSSA.ttl#Avionics>
  rdf:type owl:Class ;
  rdfs:subClassOf <http://lpis.csd.auth.gr/ontologies/2015/OoSSA.ttl#AbstractionLevel> ;
.
<http://lpis.csd.auth.gr/ontologies/2015/OoSSA.ttl#ComponentImplementation>
  rdfs:subClassOf <http://lpis.csd.auth.gr/ontologies/2015/PRP#Component> ;
.
<http://lpis.csd.auth.gr/ontologies/2015/OoSSA.ttl#Event>
  rdf:type owl:Class ;
  rdfs:subClassOf <http://lpis.csd.auth.gr/ontologies/2015/RBLP#Event> ;
.
<http://lpis.csd.auth.gr/ontologies/2015/OoSSA.ttl#Interaction>
  rdfs:subClassOf <http://lpis.csd.auth.gr/ontologies/2015/PRP#Interaction> ;
.
<http://lpis.csd.auth.gr/ontologies/2015/OoSSA.ttl#Mode>
  rdf:type owl:Class ;
  rdfs:subClassOf <http://lpis.csd.auth.gr/ontologies/2015/PRP#Mode> ;
  rdfs:subClassOf <http://lpis.csd.auth.gr/ontologies/2015/RBLP#Mode> ;
.
<http://lpis.csd.auth.gr/ontologies/2015/OoSSA.ttl#ModeChange>
  rdfs:subClassOf <http://lpis.csd.auth.gr/ontologies/2015/PRP#ModeChange> ;
.
<http://lpis.csd.auth.gr/ontologies/2015/OoSSA.ttl#PortActivation>
  rdfs:subClassOf <http://lpis.csd.auth.gr/ontologies/2015/PRP#PortActivation> ;
.
<http://lpis.csd.auth.gr/ontologies/2015/OoSSA.ttl#RB>
  rdf:type owl:Class ;
  rdfs:subClassOf <http://lpis.csd.auth.gr/ontologies/2015/OoSSA.ttl#AbstractionLevel> ;
.
<http://lpis.csd.auth.gr/ontologies/2015/OoSSA.ttl#State>
  rdf:type owl:Class ;
  rdfs:subClassOf <http://lpis.csd.auth.gr/ontologies/2015/RBLP#State> ;
.
<http://lpis.csd.auth.gr/ontologies/2015/OoSSA.ttl#SystemAction>
  rdf:type owl:Class ;
  rdfs:subClassOf <http://lpis.csd.auth.gr/ontologies/2015/RBLP#Action> ;
.
<http://lpis.csd.auth.gr/ontologies/2015/OoSSA.ttl#SystemAttribute>
  rdfs:subClassOf <http://lpis.csd.auth.gr/ontologies/2015/RBLP#Entity> ;
.
<http://lpis.csd.auth.gr/ontologies/2015/OoSSA.ttl#SystemEntity>
  rdf:type owl:Class ;
  rdfs:subClassOf <http://lpis.csd.auth.gr/ontologies/2015/RBLP#Actor> ;
.
<http://lpis.csd.auth.gr/ontologies/2015/OoSSA.ttl#SystemSpacecraft>
  rdf:type owl:Class ;
  rdfs:subClassOf <http://lpis.csd.auth.gr/ontologies/2015/OoSSA.ttl#AbstractionLevel> ;
.
<http://lpis.csd.auth.gr/ontologies/2015/OoSSA.ttl#TS>
  rdf:type owl:Class ;
  rdfs:subClassOf <http://lpis.csd.auth.gr/ontologies/2015/OoSSA.ttl#AbstractionLevel> ;
.
<http://lpis.csd.auth.gr/ontologies/2015/RBLP#M1>
  rdf:type owl:Class ;
  rdfs:comment "<system> shall [not] <action>"^^xsd:string ;
  rdfs:subClassOf <http://lpis.csd.auth.gr/ontologies/2015/RBLP#Main> ;
  rdfs:subClassOf [
      rdf:type owl:Restriction ;
      owl:allValuesFrom <http://lpis.csd.auth.gr/ontologies/2015/RBLP#Action> ;
      owl:onProperty <http://lpis.csd.auth.gr/ontologies/2015/RBLP#isRelatedToAttribute> ;
    ] ;
  rdfs:subClassOf [
      rdf:type owl:Restriction ;
      owl:cardinality "1"^^xsd:nonNegativeInteger ;
      owl:onProperty <http://lpis.csd.auth.gr/ontologies/2015/RBLP#isRelatedToAction> ;
    ] ;
  rdfs:subClassOf [
      rdf:type owl:Restriction ;
      owl:cardinality "1"^^xsd:nonNegativeInteger ;
      owl:onProperty <http://lpis.csd.auth.gr/ontologies/2015/RBLP#isRelatedToAttribute> ;
    ] ;
.
